veric/SeparationLogicSoundness.v
@@ -1,7 +1,8 @@
 Require Import VST.sepcomp.semantics.
 
 Require Import VST.veric.juicy_base.
-Require Import VST.veric.juicy_mem VST.veric.juicy_mem_lemmas VST.veric.juicy_mem_ops.
+Require Import VST.veric.juicy_mem VST.veric.juicy_mem_lemmas.
+Require Import VST.veric.external_state.
 Require Import VST.veric.res_predicates.
 Require Import VST.veric.extend_tc.
 Require Import VST.veric.Clight_seplog.
@@ -25,8 +26,6 @@ Require Import VST.veric.semax_prog.
 Require Import VST.veric.semax_ext.
 Require Import VST.veric.SeparationLogic.
 
-Require Import VST.veric.ghost_PCM.
-
 Module Type SEPARATION_HOARE_LOGIC_SOUNDNESS.
 
 Declare Module CSHL_Def: CLIGHT_SEPARATION_HOARE_LOGIC_DEF.
@@ -37,31 +36,22 @@ Import CSHL_Def.
 Import CSHL_Defs.
 
 Axiom semax_prog_sound :
-  forall {Espec: OracleKind}{CS: compspecs} prog z Vspec Gspec,
-  @semax_prog Espec CS prog z Vspec Gspec ->
-  @semax_prog.semax_prog Espec CS prog z Vspec Gspec.
+  forall `{H : heapGS Σ}{Espec: OracleKind}{HE : externalGS OK_ty Σ}{CS: compspecs} prog z Vspec Gspec,
+  @semax_prog Σ H Espec HE CS prog z Vspec Gspec ->
+  @semax_prog.semax_prog Σ H Espec HE CS prog z Vspec Gspec.
 
 Axiom semax_prog_rule :
-  forall {Espec: OracleKind}{CS: compspecs},
+  forall `{H : heapGS Σ}{Espec: OracleKind}{HE : externalGS OK_ty Σ}{CS: compspecs},
   forall V G prog m h z,
-     postcondition_allows_exit Espec tint ->
-     @semax_prog Espec CS prog z V G ->
+     @postcondition_allows_exit _ Espec tint ->
+     @semax_prog Σ H Espec HE CS prog z V G ->
      Genv.init_mem prog = Some m ->
      { b : block & { q : CC_core &
-       (Genv.find_symbol (globalenv prog) (prog_main prog) = Some b) *
-       (forall jm, m_dry jm = m -> exists jm',
-                    semantics.initial_core (juicy_core_sem (cl_core_sem (globalenv prog))) h
-                       jm q jm' (Vptr b Ptrofs.zero) nil) *
-       forall n,
-         { jm |
-           m_dry jm = m /\ level jm = n /\
-           nth_error (ghost_of (m_phi jm)) 0 = Some (Some (ext_ghost z, NoneP)) /\
-           (exists z, join (m_phi jm) (wsat_rmap (m_phi jm)) (m_phi z) /\ ext_order jm z) /\
-           jsafeN (@OK_spec Espec) (globalenv prog) z q jm /\
-           no_locks (m_phi jm) /\
-           matchfunspecs (globalenv prog) G (m_phi jm) /\
-           app_pred (funassert (nofunc_tycontext V G) (empty_environ (globalenv prog))) (m_phi jm)
-     } } }%type.
+       (exists m', semantics.initial_core (cl_core_sem (globalenv prog)) h
+                       m q m' (Vptr b Ptrofs.zero) nil) *
+       (state_interp Mem.empty z ∗ has_ext z ⊢ |==> state_interp m z ∗ jsafeN Espec (globalenv prog) ⊤ z q ∗
+           (*no_locks ∧ □ matchfunspecs (globalenv prog) G ⊤ ∗*) funassert (nofunc_tycontext V G) (empty_environ (globalenv prog)))
+     } }%type.
 
 End SEPARATION_HOARE_LOGIC_SOUNDNESS.
 
@@ -83,8 +73,7 @@ Definition semax := @semax.
 
 Definition semax_func := @semax_func.
 
-Definition semax_external {Espec: OracleKind} ef A P Q :=
-  forall n, semax_external Espec ef A P Q n.
+Definition semax_external := @semax_external.
 
 End VericDef.
 
@@ -93,7 +82,14 @@ Module VericMinimumSeparationLogic: MINIMUM_CLIGHT_SEPARATION_HOARE_LOGIC with M
 Module CSHL_Def := VericDef.
 Module CSHL_Defs := DerivedDefs (VericDef).
 
-Definition semax_extract_exists := @extract_exists_pre.
+Lemma semax_extract_exists: forall `{!heapGS Σ} Espec `{!externalGS OK_ty Σ} {CS: compspecs} E (A : Type) (P : A -> assert) c (Delta: tycontext) (R: ret_assert),
+  (forall x, semax Espec E Delta (P x) c R) ->
+   semax Espec E Delta (∃ x:A, P x) c R.
+Proof.
+  intros; eapply semax_pre, extract_exists_pre, H.
+  intros; rewrite bi.and_elim_r; monPred.unseal; done.
+Qed.
+
 Definition semax_body := @semax_body.
 Definition semax_prog := @semax_prog.
 Definition semax_func_nil := @semax_func_nil.
@@ -101,29 +97,28 @@ Definition semax_func_cons := @semax_func_cons.
 Definition make_ext_rval := veric.semax.make_ext_rval.
 Definition tc_option_val := veric.semax.tc_option_val.
 
-Lemma semax_func_cons_ext: forall {Espec:OracleKind} (V: varspecs) (G: funspecs)
-     {C: compspecs} ge fs id ef argsig retsig A P Q NEP NEQ argsig'
+Lemma semax_func_cons_ext: forall `{HH: heapGS Σ}{Espec:OracleKind}{HE: externalGS OK_ty Σ} (V: varspecs) (G: funspecs)
+     {C: compspecs} ge E fs id ef argsig retsig A P Q argsig'
       (G': funspecs) cc b,
   argsig' = typelist2list argsig ->
   ef_sig ef = mksignature (typlist_of_typelist argsig) (rettype_of_type retsig) cc ->
   id_in_list id (map (@fst _ _) fs) = false ->
   (ef_inline ef = false \/ withtype_empty A) ->
-  (forall gx ts x (ret : option val),
-      (seplog.derives (seplog.andp
-                         (Q ts x (make_ext_rval gx (rettype_of_type retsig) ret))
-                         (!! Builtins0.val_opt_has_rettype ret (rettype_of_type retsig)))
-                      (!!tc_option_val retsig ret))) ->
+  (forall gx x (ret : option val),
+      Q x (make_ext_rval gx (rettype_of_type retsig) ret) ∧
+      ⌜Builtins0.val_opt_has_rettype ret (rettype_of_type retsig)⌝ ⊢
+      ⌜tc_option_val retsig ret⌝) ->
   Genv.find_symbol ge id = Some b ->
   Genv.find_funct_ptr ge b = Some (Ctypes.External ef argsig retsig cc) ->
-  @CSHL_Def.semax_external Espec ef A P Q ->
-  CSHL_Def.semax_func Espec V G C ge fs G' ->
-  CSHL_Def.semax_func Espec V G C ge ((id, Ctypes.External ef argsig retsig cc)::fs)
-             ((id, mk_funspec (argsig', retsig) cc A P Q NEP NEQ)  :: G').
-Proof. intros. eapply semax_func_cons_ext; eauto. intros. apply H3. Qed.
+  (⊢ @CSHL_Def.semax_external _ HH Espec HE E ef A P Q) ->
+  CSHL_Def.semax_func _ HH Espec HE V G C ge E fs G' ->
+  CSHL_Def.semax_func _ HH Espec HE V G C ge E ((id, Ctypes.External ef argsig retsig cc)::fs)
+             ((id, mk_funspec (argsig', retsig) cc A P Q)  :: G').
+Proof. intros. eapply semax_func_cons_ext; eauto. Qed.
 
 Definition semax_Delta_subsumption := @semax_lemmas.semax_Delta_subsumption.
 
-Lemma semax_external_binaryintersection: forall
+(*Lemma semax_external_binaryintersection: forall
  {Espec ef A1 P1 Q1 P1ne Q1ne A2 P2 Q2 P2ne Q2ne A P Q P_ne Q_ne sig cc}
   (EXT1: @CSHL_Def.semax_external Espec ef A1 P1 Q1)
   (EXT2: @CSHL_Def.semax_external Espec ef A2 P2 Q2)
@@ -132,121 +127,119 @@ Lemma semax_external_binaryintersection: forall
      Some (mk_funspec sig cc A P Q P_ne Q_ne))
   (LEN: length (fst sig) = length (sig_args (ef_sig ef))),
   @CSHL_Def.semax_external Espec ef A P Q. 
-Proof. intros. intros n. eapply semax_external_binaryintersection. apply EXT1. apply EXT2. apply BI. trivial. Qed.
+Proof. intros. intros n. eapply semax_external_binaryintersection. apply EXT1. apply EXT2. apply BI. trivial. Qed.*)
 
-Lemma semax_external_funspec_sub: forall 
-  (DISABLE: False) {Espec argtypes rtype cc ef A1 P1 Q1 P1ne Q1ne A P Q Pne Qne}
-  (Hsub: funspec_sub (mk_funspec (argtypes, rtype) cc A1 P1 Q1 P1ne Q1ne) 
-                   (mk_funspec (argtypes, rtype) cc A P Q Pne Qne))
-  (HSIG: ef_sig ef = 
+Lemma semax_external_funspec_sub: forall `{HH : heapGS Σ}
+  {Espec HE E argtypes rtype cc ef A1 P1 Q1 A P Q}
+  (Hsub: funspec_sub E (mk_funspec (argtypes, rtype) cc A1 P1 Q1)
+                   (mk_funspec (argtypes, rtype) cc A P Q))
+  (HSIG: ef_sig ef =
          mksignature (map typ_of_type argtypes)
-                     (rettype_of_type rtype) cc)
-  (SE: @CSHL_Def.semax_external Espec ef A1 P1 Q1),
-  @CSHL_Def.semax_external Espec ef A P Q.
+                     (rettype_of_type rtype) cc),
+  @CSHL_Def.semax_external _ HH Espec HE E ef A1 P1 Q1 ⊢
+  @CSHL_Def.semax_external _ HH Espec HE E ef A P Q.
 Proof.
-  intros. intros n. eapply semax_external_funspec_sub.
-  assumption.
-  rewrite <- funspec_sub_iff. apply Hsub. trivial. trivial.
+  intros. eapply semax_external_funspec_sub; eauto.
 Qed.
 
-Definition semax_body_binaryintersection := @semax_body_binaryintersection.
+(*Definition semax_body_binaryintersection := @semax_body_binaryintersection.*)
 
-Definition semax_func_mono := semax_func_mono.
-Definition semax_func_app := semax_func_app.
-Definition semax_func_subsumption := semax_func_subsumption.
-Definition semax_func_join  := semax_func_join.
-Definition semax_func_firstn := semax_func_firstn.
-Definition semax_func_skipn := semax_func_skipn.
-Definition semax_body_subsumption:= semax_body_subsumption.
-Definition semax_body_cenv_sub:= @semax_body_cenv_sub.
+Definition semax_func_mono := @semax_func_mono.
+Definition semax_func_app := @semax_func_app.
+Definition semax_func_subsumption := @semax_func_subsumption.
+Definition semax_func_join  := @semax_func_join.
+Definition semax_func_firstn := @semax_func_firstn.
+Definition semax_func_skipn := @semax_func_skipn.
+Definition semax_body_subsumption := @semax_body_subsumption.
+Definition semax_body_cenv_sub := @semax_body_cenv_sub.
 
 Lemma semax_body_funspec_sub:
-  forall (V : varspecs) (G : funspecs) (cs : compspecs) (f : function) 
+  forall `{!heapGS Σ} {Espec : OracleKind} `{!externalGS OK_ty Σ} (V : varspecs) (G : funspecs) (cs : compspecs) E (f : function) 
    (i : ident) (phi phi' : funspec),
- CSHL_Defs.semax_body V G f (i, phi) ->
- funspec_sub phi phi' ->
+ CSHL_Defs.semax_body V G E f (i, phi) ->
+ funspec_sub E phi phi' ->
  list_norepet (map fst (fn_params f) ++ map fst (fn_temps f)) ->
- CSHL_Defs.semax_body V G f (i, phi').
+ CSHL_Defs.semax_body V G E f (i, phi').
 Proof.
-  intros. eapply semax_body_funspec_sub; eauto. now rewrite <- funspec_sub_iff.
+  intros. eapply semax_body_funspec_sub; eauto.
 Qed.
 
 Definition semax_seq := @semax_seq.
 Definition semax_break := @semax_break.
 Definition semax_continue := @semax_continue.
 Definition semax_loop := @semax_loop.
-Definition semax_switch := @semax_switch.
+
+Lemma semax_switch : forall `{HH: heapGS Σ}{Espec:OracleKind}{HE: externalGS OK_ty Σ}{CS: compspecs}
+  E Delta (Q: assert) a sl R,
+     is_int_type (typeof a) = true ->
+     (forall rho, Q rho ⊢ tc_expr Delta a rho) ->
+     (forall n,
+     semax Espec E Delta 
+               (local (liftx eq (eval_expr a) (liftx (Vint n))) ∧ Q)
+               (seq_of_labeled_statement (select_switch (Int.unsigned n) sl))
+               (switch_ret_assert R)) ->
+     semax Espec E Delta Q (Sswitch a sl) R.
+Proof.
+  intros; eapply semax_switch; try done.
+  intros; eapply semax_pre, H1.
+  intros; rewrite bi.and_elim_r; monPred.unseal; done.
+Qed.
+
 Definition semax_Slabel := @semax_Slabel.
 Definition semax_set_forward := @semax_set_forward.
 Definition semax_ifthenelse := @semax_ifthenelse.
-Definition semax_return := @semax_return.
 
-Import VST.msl.seplog VST.veric.lift.
+Lemma semax_return `{HH : !heapGS Σ} {Espec} `{HE : !externalGS OK_ty Σ} {CS}:
+   forall E Delta (R: ret_assert) ret,
+      semax Espec E Delta
+                (tc_expropt Delta ret (ret_type Delta) ∧
+                (assert_of (liftx (RA_return R : option val -> environ -> mpred) (cast_expropt ret (ret_type Delta)) (@id environ))))
+                (Sreturn ret)
+                R.
+Proof.
+  intros; eapply semax_pre, semax_return.
+  intros; rewrite bi.and_elim_r; monPred.unseal; done.
+Qed.
 
-Lemma semax_call {CS Espec}:
-  forall Delta (A: TypeTree)
-  (P : forall ts, dependent_type_functor_rec ts (ArgsTT A) mpred)
-  (Q : forall ts, dependent_type_functor_rec ts (AssertTT A) mpred)
-  (NEP: args_super_non_expansive P) (NEQ: super_non_expansive Q)
-  (ts: list Type) (x : dependent_type_functor_rec ts A mpred)
-   F ret argsig retsig cc a bl,
+(* Why are the implicits so inconsistent here? *)
+Lemma semax_call `{HH : !heapGS Σ} {Espec} `{HE : !externalGS OK_ty Σ} {CS}:
+  forall E Delta (A: Type)
+  (P : A -> argsEnviron -> mpred)
+  (Q : A -> environ -> mpred)
+  (x : A)
+   F ret id argsig retsig cc a bl,
            Cop.classify_fun (typeof a) =
            Cop.fun_case_f (typelist_of_type_list argsig) retsig cc ->
             (retsig = Ctypes.Tvoid -> ret = None) ->
           tc_fn_return Delta ret retsig ->
-  @semax CS Espec Delta
-       (fun rho => ((tc_expr Delta a rho && tc_exprlist Delta argsig bl rho))  &&
-           (func_ptr (mk_funspec (argsig,retsig) cc A P Q NEP NEQ) (eval_expr a rho) &&
-          (|>(F rho * P ts x (ge_of rho, eval_exprlist argsig bl rho)))))%pred
+  @semax _ HH Espec HE CS E Delta
+       ((tc_expr Delta a ∧ tc_exprlist Delta argsig bl) ∧
+         (assert_of (fun rho => func_ptr (ge_of rho) E id (mk_funspec (argsig,retsig) cc A P Q) (eval_expr a rho)) ∗
+          (▷(F ∗ assert_of (fun rho => P x (ge_of rho, eval_exprlist argsig bl rho))))))
          (Scall ret a bl)
-         (normal_ret_assert
-            (@exp
-               (forall _ : environ,
-                functors.MixVariantFunctor._functor functors.MixVariantFunctorGenerator.fidentity
-                  mpred)
-               (@LiftNatDed'
-                  (functors.MixVariantFunctor._functor
-                     functors.MixVariantFunctorGenerator.fidentity mpred) Nveric) val
-               (fun old : val =>
-                @sepcon
-                  (forall _ : environ,
-                   functors.MixVariantFunctor._functor
-                     functors.MixVariantFunctorGenerator.fidentity mpred)
-                  (@LiftNatDed'
-                     (functors.MixVariantFunctor._functor
-                        functors.MixVariantFunctorGenerator.fidentity mpred) Nveric)
-                  (@LiftSepLog'
-                     (functors.MixVariantFunctor._functor
-                        functors.MixVariantFunctorGenerator.fidentity mpred) Nveric Sveric)
-                  (@substopt
-                     (functors.MixVariantFunctor._functor
-                        functors.MixVariantFunctorGenerator.fidentity mpred) ret
-                     (@liftx (LiftEnviron val) old) F) (maybe_retval (Q ts x) retsig ret)))).
+         (normal_ret_assert (∃ old:val, assert_of (substopt ret (liftx old) F) ∗ maybe_retval (Q x) retsig ret)).
 Proof.
-  intros. specialize (@semax_call_si CS Espec Delta A P Q NEP NEQ ts x F ret argsig retsig cc a bl H H0 H1); intros X.
-  eapply semax_pre; [| apply X].
-  intros. simpl. intros w [TC [W1 W2]]; split; trivial.
-  eapply predicates_hered.now_later. rewrite <- tc_expr_eq; apply W1.
-Qed. 
+  intros. eapply semax_pre_post, semax_call_si; try done; [| by intros; rewrite bi.and_elim_r; monPred.unseal..].
+  intros; rewrite bi.and_elim_r; monPred.unseal; apply bi.and_mono; [apply bi.later_intro | done].
+Qed.
 
-Lemma semax_store:forall (CS : compspecs) (Espec : OracleKind) 
-         (Delta : tycontext) (e1 e2 : expr) (sh : share)
-         (P : environ -> pred rmap),
+Lemma semax_store: forall `{HH : !heapGS Σ} (CS : compspecs) (Espec : OracleKind) `{HE : !externalGS OK_ty Σ}
+         E (Delta : tycontext) (e1 e2 : expr) (sh : share)
+         (P : environ -> mpred),
        writable_share sh ->
-       semax Espec Delta
+       semax Espec E Delta
          (fun rho : environ =>
-          (|> (extend_tc.tc_lvalue Delta e1 rho &&
-               extend_tc.tc_expr Delta (Ecast e2 (typeof e1)) rho &&
-               (mapsto_memory_block.mapsto_ sh 
-                  (typeof e1) (eval_lvalue e1 rho) * 
-                P rho)))%pred) (Sassign e1 e2)
-         (Clight_seplog.normal_ret_assert
+          (▷ (tc_lvalue Delta e1 rho ∧
+              tc_expr Delta (Ecast e2 (typeof e1)) rho ∧
+               (mapsto_ sh (typeof e1) (eval_lvalue e1 rho) ∗
+                P rho)))) (Sassign e1 e2)
+         (normal_ret_assert
             (fun rho : environ =>
              (mapsto_memory_block.mapsto sh (typeof e1)
                 (eval_lvalue e1 rho)
                 (force_val
-                   (sem_cast (typeof e2) (typeof e1) (eval_expr e2 rho))) *
-              P rho)%pred)).
+                   (sem_cast (typeof e2) (typeof e1) (eval_expr e2 rho))) ∗
+              P rho))).
 Proof.
 intros; apply semax_store; auto.
 Qed.
@@ -261,7 +254,7 @@ Definition semax_conseq := @semax_conseq.
 Definition semax_ptr_compare := @semax_ptr_compare.
 Definition semax_external_FF := @semax_external_FF.
 
-Definition juicy_ext_spec := juicy_ext_spec.
+Definition juicy_ext_spec := @juicy_ext_spec.
 
 Definition semax_ext := @semax_ext.
 
@@ -273,9 +266,9 @@ Module CSHL_Def := VericDef.
 Module CSHL_Defs := DerivedDefs (VericDef).
 
 Lemma semax_prog_sound :
-  forall {Espec}{CS} prog z Vspec Gspec,
-  @CSHL_Defs.semax_prog Espec CS prog z Vspec Gspec ->
-  @semax_prog.semax_prog Espec CS prog z Vspec Gspec.
+  forall `{HH : heapGS Σ}{Espec}{HE : externalGS OK_ty Σ}{CS} prog z Vspec Gspec,
+  @CSHL_Defs.semax_prog _ HH Espec HE CS prog z Vspec Gspec ->
+  @semax_prog.semax_prog _ HH Espec HE CS prog z Vspec Gspec.
 Proof.
   intros; apply H.
 Qed.
